POPL24

coq/theories/logical_ctx.v
@@ -1,3 +1,5 @@
+(* This file defines the logical context (Γ). *)
+
 From mathcomp Require Import ssreflect ssrbool eqtype ssrnat seq.
 From Coq Require Import ssrfun Classical Utf8.
 Require Import AutosubstSsr ARS tll_ast.
@@ -6,15 +8,15 @@ Set Implicit Arguments.
 Unset Strict Implicit.
 Unset Printing Implicit Defensive.
 
-Definition sta_ctx := seq term.
+Definition logical_ctx := seq term.
 
-Inductive sta_has :
-  sta_ctx -> var -> term -> Prop :=
-| sta_has_O Γ A :
-  sta_has (A :: Γ) 0 A.[ren (+1)]
-| sta_has_S Γ A B x :
-  sta_has Γ x A ->
-  sta_has (B :: Γ) x.+1 A.[ren (+1)].
+Inductive logical_has :
+  logical_ctx -> var -> term -> Prop :=
+| logical_has_O Γ A :
+  logical_has (A :: Γ) 0 A.[ren (+1)]
+| logical_has_S Γ A B x :
+  logical_has Γ x A ->
+  logical_has (B :: Γ) x.+1 A.[ren (+1)].
 
-Lemma sta_has_size Γ x A : sta_has Γ x A -> x < size Γ.
+Lemma logical_has_size Γ x A : logical_has Γ x A -> x < size Γ.
 Proof. elim=>//. Qed.
