coq/theories/logical_conf.v
@@ -1,11 +1,15 @@
+(* This file presents the confluence theorem for the logical level
+   and various congruence lemmas and corollaries of confluence. *)
+
 From mathcomp Require Import ssreflect ssrbool eqtype ssrnat seq.
 From Coq Require Import ssrfun Classical Utf8.
-Require Export AutosubstSsr ARS sta_step.
+Require Export AutosubstSsr ARS logical_step.
 
 Set Implicit Arguments.
 Unset Strict Implicit.
 Unset Printing Implicit Defensive.
 
+(* Parallel reduction for the logical level. *)
 Inductive pstep : term -> term -> Prop :=
 | pstep_var x :
   pstep (Var x) (Var x)
@@ -111,190 +115,190 @@ Inductive pstep : term -> term -> Prop :=
 
 Definition sred σ τ := forall x : var, (σ x) ~>* (τ x).
 
-Lemma sta_step_subst σ m n : m ~> n -> m.[σ] ~> n.[σ].
+Lemma logical_step_subst σ m n : m ~> n -> m.[σ] ~> n.[σ].
 Proof.
-  move=> st. elim: st σ=>/={m n}; eauto using sta_step.
+  move=> st. elim: st σ=>/={m n}; eauto using logical_step.
   { move=> A m n s σ.
     replace (m.[n/].[σ]) with (m.[up σ].[n.[σ]/]).
-    apply sta_step_beta0. autosubst. }
+    apply logical_step_beta0. autosubst. }
   { move=> A m n s σ.
     replace (m.[n/].[σ]) with (m.[up σ].[n.[σ]/]).
-    apply sta_step_beta1. autosubst. }
+    apply logical_step_beta1. autosubst. }
   { move=>A m1 m2 n s σ.
     replace (n.[m2,m1/].[σ]) with (n.[upn 2 σ].[m2.[σ],m1.[σ]/]).
-    apply: sta_step_iota0. autosubst. }
+    apply: logical_step_iota0. autosubst. }
   { move=>A m1 m2 n s σ.
     replace (n.[m2,m1/].[σ]) with (n.[upn 2 σ].[m2.[σ],m1.[σ]/]).
-    apply: sta_step_iota1. autosubst. }
+    apply: logical_step_iota1. autosubst. }
 Qed.
 
-Lemma sta_red_app m m' n n' :
+Lemma logical_red_app m m' n n' :
   m ~>* m' -> n ~>* n' -> App m n ~>* App m' n'.
 Proof.
   move=> r1 r2.
   apply: (star_trans (App m' n)).
-  apply: (star_hom (App^~ n)) r1=>x y. exact: sta_step_appL.
-  apply: star_hom r2. exact: sta_step_appR.
+  apply: (star_hom (App^~ n)) r1=>x y. exact: logical_step_appL.
+  apply: star_hom r2. exact: logical_step_appR.
 Qed.
 
-Lemma sta_red_lam0 A A' m m' s :
+Lemma logical_red_lam0 A A' m m' s :
   A ~>* A' -> m ~>* m' -> Lam0 A m s ~>* Lam0 A' m' s.
 Proof.
   move=> r1 r2.
   apply: (star_trans (Lam0 A' m s)).
-  apply: (star_hom ((Lam0^~ m)^~ s)) r1=>x y. exact: sta_step_lam0L.
-  apply: (star_hom ((Lam0 A')^~ s)) r2=>x y. exact: sta_step_lam0R.
+  apply: (star_hom ((Lam0^~ m)^~ s)) r1=>x y. exact: logical_step_lam0L.
+  apply: (star_hom ((Lam0 A')^~ s)) r2=>x y. exact: logical_step_lam0R.
 Qed.
 
-Lemma sta_red_lam1 A A' m m' s :
+Lemma logical_red_lam1 A A' m m' s :
   A ~>* A' -> m ~>* m' -> Lam1 A m s ~>* Lam1 A' m' s.
 Proof.
   move=> r1 r2.
   apply: (star_trans (Lam1 A' m s)).
-  apply: (star_hom ((Lam1^~ m)^~ s)) r1=>x y. exact: sta_step_lam1L.
-  apply: (star_hom ((Lam1 A')^~ s)) r2=>x y. exact: sta_step_lam1R.
+  apply: (star_hom ((Lam1^~ m)^~ s)) r1=>x y. exact: logical_step_lam1L.
+  apply: (star_hom ((Lam1 A')^~ s)) r2=>x y. exact: logical_step_lam1R.
 Qed.
 
-Lemma sta_red_pi0 A A' B B' s :
+Lemma logical_red_pi0 A A' B B' s :
   A ~>* A' -> B ~>* B' -> Pi0 A B s ~>* Pi0 A' B' s.
 Proof.
   move=> r1 r2.
   apply: (star_trans (Pi0 A' B s)).
-  apply: (star_hom ((Pi0^~ B)^~ s)) r1=>x y. exact: sta_step_pi0L.
-  apply: (star_hom ((Pi0 A')^~ s)) r2=>x y. exact: sta_step_pi0R.
+  apply: (star_hom ((Pi0^~ B)^~ s)) r1=>x y. exact: logical_step_pi0L.
+  apply: (star_hom ((Pi0 A')^~ s)) r2=>x y. exact: logical_step_pi0R.
 Qed.
 
-Lemma sta_red_pi1 A A' B B' s :
+Lemma logical_red_pi1 A A' B B' s :
   A ~>* A' -> B ~>* B' -> Pi1 A B s ~>* Pi1 A' B' s.
 Proof.
   move=> r1 r2.
   apply: (star_trans (Pi1 A' B s)).
-  apply: (star_hom ((Pi1^~ B)^~ s)) r1=>x y. exact: sta_step_pi1L.
-  apply: (star_hom ((Pi1 A')^~ s)) r2=>x y. exact: sta_step_pi1R.
+  apply: (star_hom ((Pi1^~ B)^~ s)) r1=>x y. exact: logical_step_pi1L.
+  apply: (star_hom ((Pi1 A')^~ s)) r2=>x y. exact: logical_step_pi1R.
 Qed.
 
-Lemma sta_red_sig0 A A' B B' s :
+Lemma logical_red_sig0 A A' B B' s :
   A ~>* A' -> B ~>* B' -> Sig0 A B s ~>* Sig0 A' B' s.
 Proof.
   move=> r1 r2.
   apply: (star_trans (Sig0 A' B s)).
-  apply: (star_hom ((Sig0^~ B)^~ s)) r1=>x y. exact: sta_step_sig0L.
-  apply: (star_hom ((Sig0 A')^~ s)) r2=>x y. exact: sta_step_sig0R.
+  apply: (star_hom ((Sig0^~ B)^~ s)) r1=>x y. exact: logical_step_sig0L.
+  apply: (star_hom ((Sig0 A')^~ s)) r2=>x y. exact: logical_step_sig0R.
 Qed.
 
-Lemma sta_red_sig1 A A' B B' s :
+Lemma logical_red_sig1 A A' B B' s :
   A ~>* A' -> B ~>* B' -> Sig1 A B s ~>* Sig1 A' B' s.
 Proof.
   move=> r1 r2.
   apply: (star_trans (Sig1 A' B s)).
-  apply: (star_hom ((Sig1^~ B)^~ s)) r1=>x y. exact: sta_step_sig1L.
-  apply: (star_hom ((Sig1 A')^~ s)) r2=>x y. exact: sta_step_sig1R.
+  apply: (star_hom ((Sig1^~ B)^~ s)) r1=>x y. exact: logical_step_sig1L.
+  apply: (star_hom ((Sig1 A')^~ s)) r2=>x y. exact: logical_step_sig1R.
 Qed.
 
-Lemma sta_red_pair0 m m' n n' t :
+Lemma logical_red_pair0 m m' n n' t :
   m ~>* m' -> n ~>* n' -> Pair0 m n t ~>* Pair0 m' n' t.
 Proof.
   move=>r1 r2.
   apply: (star_trans (Pair0 m' n t)).
-  apply: (star_hom ((Pair0^~ n)^~ t)) r1=>x y. exact: sta_step_pair0L.
-  apply: (star_hom ((Pair0 m')^~ t)) r2=>x y. exact: sta_step_pair0R.
+  apply: (star_hom ((Pair0^~ n)^~ t)) r1=>x y. exact: logical_step_pair0L.
+  apply: (star_hom ((Pair0 m')^~ t)) r2=>x y. exact: logical_step_pair0R.
 Qed.
 
-Lemma sta_red_pair1 m m' n n' t :
+Lemma logical_red_pair1 m m' n n' t :
   m ~>* m' -> n ~>* n' -> Pair1 m n t ~>* Pair1 m' n' t.
 Proof.
   move=>r1 r2.
   apply: (star_trans (Pair1 m' n t)).
-  apply: (star_hom ((Pair1^~ n)^~ t)) r1=>x y. exact: sta_step_pair1L.
-  apply: (star_hom ((Pair1 m')^~ t)) r2=>x y. exact: sta_step_pair1R.
+  apply: (star_hom ((Pair1^~ n)^~ t)) r1=>x y. exact: logical_step_pair1L.
+  apply: (star_hom ((Pair1 m')^~ t)) r2=>x y. exact: logical_step_pair1R.
 Qed.
 
-Lemma sta_red_letin A A' m m' n n' :
+Lemma logical_red_letin A A' m m' n n' :
   A ~>* A' -> m ~>* m' -> n ~>* n' -> LetIn A m n ~>* LetIn A' m' n'.
 Proof.
   move=>r1 r2 r3.
   apply: (star_trans (LetIn A' m n)).
-  apply: (star_hom ((LetIn^~ m)^~ n)) r1=>x y. exact: sta_step_letinA.
+  apply: (star_hom ((LetIn^~ m)^~ n)) r1=>x y. exact: logical_step_letinA.
   apply: (star_trans (LetIn A' m' n)).
-  apply: (star_hom (LetIn A'^~ n)) r2=>x y. exact: sta_step_letinL.
-  apply: (star_hom (LetIn A' m')) r3=>x y. exact: sta_step_letinR.
+  apply: (star_hom (LetIn A'^~ n)) r2=>x y. exact: logical_step_letinL.
+  apply: (star_hom (LetIn A' m')) r3=>x y. exact: logical_step_letinR.
 Qed.
 
-Lemma sta_red_with A A' B B' s :
+Lemma logical_red_with A A' B B' s :
   A ~>* A' -> B ~>* B' -> With A B s ~>* With A' B' s.
 Proof.
   move=>r1 r2.
   apply: (star_trans (With A' B s)).
-  apply: (star_hom ((With^~ B)^~ s)) r1=>x y. exact: sta_step_withL.
-  apply: (star_hom ((With A')^~ s)) r2=>x y. exact: sta_step_withR.
+  apply: (star_hom ((With^~ B)^~ s)) r1=>x y. exact: logical_step_withL.
+  apply: (star_hom ((With A')^~ s)) r2=>x y. exact: logical_step_withR.
 Qed.
 
-Lemma sta_red_apair m m' n n' s :
+Lemma logical_red_apair m m' n n' s :
   m ~>* m' -> n ~>* n' -> APair m n s ~>* APair m' n' s.
 Proof.
   move=>r1 r2.
   apply: (star_trans (APair m' n s)).
-  apply: (star_hom ((APair^~ n)^~ s)) r1=>x y. exact: sta_step_apairL.
-  apply: (star_hom ((APair m')^~ s)) r2=>x y. exact: sta_step_apairR.
+  apply: (star_hom ((APair^~ n)^~ s)) r1=>x y. exact: logical_step_apairL.
+  apply: (star_hom ((APair m')^~ s)) r2=>x y. exact: logical_step_apairR.
 Qed.
 
-Lemma sta_red_fst m m' :
+Lemma logical_red_fst m m' :
   m ~>* m' -> Fst m ~>* Fst m'.
 Proof.
   move=>r.
-  apply: (star_hom Fst) r=>x y. exact: sta_step_fst.
+  apply: (star_hom Fst) r=>x y. exact: logical_step_fst.
 Qed.
 
-Lemma sta_red_snd m m' :
+Lemma logical_red_snd m m' :
   m ~>* m' -> Snd m ~>* Snd m'.
 Proof.
   move=>r.
-  apply: (star_hom Snd) r=>x y. exact: sta_step_snd.
+  apply: (star_hom Snd) r=>x y. exact: logical_step_snd.
 Qed.
 
-Lemma sta_red_id A A' m m' n n' :
+Lemma logical_red_id A A' m m' n n' :
   A ~>* A' -> m ~>* m' -> n ~>* n' -> Id A m n ~>* Id A' m' n'.
 Proof.
   move=>r1 r2 r3.
   apply: (star_trans (Id A' m n)).
-  apply: (star_hom ((Id^~ m)^~ n)) r1=>x y. exact: sta_step_idA.
+  apply: (star_hom ((Id^~ m)^~ n)) r1=>x y. exact: logical_step_idA.
   apply: (star_trans (Id A' m' n)).
-  apply: (star_hom (Id A'^~ n)) r2=>x y. exact: sta_step_idL.
-  apply: (star_hom (Id A' m')) r3=>x y. exact: sta_step_idR.
+  apply: (star_hom (Id A'^~ n)) r2=>x y. exact: logical_step_idL.
+  apply: (star_hom (Id A' m')) r3=>x y. exact: logical_step_idR.
 Qed.
 
-Lemma sta_red_refl m m' :
+Lemma logical_red_refl m m' :
   m ~>* m' -> Refl m ~>* Refl m'.
 Proof.
   move=>r.
-  apply: (star_hom Refl) r=>x y. exact: sta_step_refl.
+  apply: (star_hom Refl) r=>x y. exact: logical_step_refl.
 Qed.
 
-Lemma sta_red_rw A A' H H' P P' :
+Lemma logical_red_rw A A' H H' P P' :
   A ~>* A' -> H ~>* H' -> P ~>* P' -> Rw A H P ~>* Rw A' H' P'.
 Proof.
   move=>r1 r2 r3.
   apply: (star_trans (Rw A' H P)).
-  apply: (star_hom ((Rw^~ H)^~ P)) r1=>x y. exact: sta_step_rwA.
+  apply: (star_hom ((Rw^~ H)^~ P)) r1=>x y. exact: logical_step_rwA.
   apply: (star_trans (Rw A' H' P)).
-  apply: (star_hom (Rw A'^~P)) r2=>x y. exact: sta_step_rwH.
-  apply: (star_hom (Rw A' H')) r3=>x y. exact: sta_step_rwP.
+  apply: (star_hom (Rw A'^~P)) r2=>x y. exact: logical_step_rwH.
+  apply: (star_hom (Rw A' H')) r3=>x y. exact: logical_step_rwP.
 Qed.
 
-Lemma sta_red_subst m n σ : m ~>* n -> m.[σ] ~>* n.[σ].
+Lemma logical_red_subst m n σ : m ~>* n -> m.[σ] ~>* n.[σ].
 Proof.
   move=>st.
   elim: st σ=>{n}; eauto.
   move=> n n' r ih st σ.
   move:(ih σ)=>{}ih.
-  move:(sta_step_subst σ st)=>r'.
+  move:(logical_step_subst σ st)=>r'.
   apply: star_trans.
   apply: ih.
   by apply: star1.
 Qed.
 
 Lemma sred_up σ τ : sred σ τ -> sred (up σ) (up τ).
-Proof. move=> A [|n] //=. asimpl. apply: sta_red_subst. exact: A. Qed.
+Proof. move=> A [|n] //=. asimpl. apply: logical_red_subst. exact: A. Qed.
 
 Lemma sred_upn n σ τ : sred σ τ -> sred (upn n σ) (upn n τ).
 Proof.
@@ -304,185 +308,185 @@ Proof.
 Qed.
 
 #[global] Hint Resolve
-  sta_red_app
-  sta_red_lam0 sta_red_lam1
-  sta_red_pi0 sta_red_pi1
-  sta_red_sig0 sta_red_sig1
-  sta_red_pair0 sta_red_pair1
-  sta_red_letin
-  sta_red_with sta_red_apair
-  sta_red_fst sta_red_snd
-  sta_red_id sta_red_refl sta_red_rw
-  sred_up sred_upn : sta_red_congr.
+  logical_red_app
+  logical_red_lam0 logical_red_lam1
+  logical_red_pi0 logical_red_pi1
+  logical_red_sig0 logical_red_sig1
+  logical_red_pair0 logical_red_pair1
+  logical_red_letin
+  logical_red_with logical_red_apair
+  logical_red_fst logical_red_snd
+  logical_red_id logical_red_refl logical_red_rw
+  sred_up sred_upn : logical_red_congr.
 
-Lemma sta_red_compat σ τ s : sred σ τ -> sta_red s.[σ] s.[τ].
-Proof. elim: s σ τ => *; asimpl; eauto 9 with sta_red_congr. Qed.
+Lemma logical_red_compat σ τ s : sred σ τ -> logical_red s.[σ] s.[τ].
+Proof. elim: s σ τ => *; asimpl; eauto 9 with logical_red_congr. Qed.
 
 Definition sconv (σ τ : var -> term) := forall x, σ x === τ x.
 
-Lemma sta_conv_app m m' n n' :
+Lemma logical_conv_app m m' n n' :
   m === m' -> n === n' -> App m n === App m' n'.
 Proof.
   move=> r1 r2.
   apply: (conv_trans (App m' n)).
-  apply: (conv_hom (App^~ n)) r1=>x y. exact: sta_step_appL.
-  apply: conv_hom r2. exact: sta_step_appR.
+  apply: (conv_hom (App^~ n)) r1=>x y. exact: logical_step_appL.
+  apply: conv_hom r2. exact: logical_step_appR.
 Qed.
 
-Lemma sta_conv_lam0 A A' m m' s :
+Lemma logical_conv_lam0 A A' m m' s :
   A === A' -> m === m' -> Lam0 A m s === Lam0 A' m' s.
 Proof.
   move=> r1 r2.
   apply: (conv_trans (Lam0 A' m s)).
-  apply: (conv_hom ((Lam0^~ m)^~ s)) r1=>x y. exact: sta_step_lam0L.
-  apply: (conv_hom ((Lam0 A')^~ s)) r2=>x y. exact: sta_step_lam0R.
+  apply: (conv_hom ((Lam0^~ m)^~ s)) r1=>x y. exact: logical_step_lam0L.
+  apply: (conv_hom ((Lam0 A')^~ s)) r2=>x y. exact: logical_step_lam0R.
 Qed.
 
-Lemma sta_conv_lam1 A A' m m' s :
+Lemma logical_conv_lam1 A A' m m' s :
   A === A' -> m === m' -> Lam1 A m s === Lam1 A' m' s.
 Proof.
   move=> r1 r2.
   apply: (conv_trans (Lam1 A' m s)).
-  apply: (conv_hom ((Lam1^~ m)^~ s)) r1=>x y. exact: sta_step_lam1L.
-  apply: (conv_hom ((Lam1 A')^~ s)) r2=>x y. exact: sta_step_lam1R.
+  apply: (conv_hom ((Lam1^~ m)^~ s)) r1=>x y. exact: logical_step_lam1L.
+  apply: (conv_hom ((Lam1 A')^~ s)) r2=>x y. exact: logical_step_lam1R.
 Qed.
 
-Lemma sta_conv_pi0 A A' B B' s :
+Lemma logical_conv_pi0 A A' B B' s :
   A === A' -> B === B' -> Pi0 A B s === Pi0 A' B' s.
 Proof.
   move=> r1 r2.
   apply: (conv_trans (Pi0 A' B s)).
-  apply: (conv_hom ((Pi0^~ B)^~ s)) r1=>x y. exact: sta_step_pi0L.
-  apply: (conv_hom ((Pi0 A')^~ s)) r2=>x y. exact: sta_step_pi0R.
+  apply: (conv_hom ((Pi0^~ B)^~ s)) r1=>x y. exact: logical_step_pi0L.
+  apply: (conv_hom ((Pi0 A')^~ s)) r2=>x y. exact: logical_step_pi0R.
 Qed.
 
-Lemma sta_conv_pi1 A A' B B' s :
+Lemma logical_conv_pi1 A A' B B' s :
   A === A' -> B === B' -> Pi1 A B s === Pi1 A' B' s.
 Proof.
   move=> r1 r2.
   apply: (conv_trans (Pi1 A' B s)).
-  apply: (conv_hom ((Pi1^~ B)^~ s)) r1=>x y. exact: sta_step_pi1L.
-  apply: (conv_hom ((Pi1 A')^~ s)) r2=>x y. exact: sta_step_pi1R.
+  apply: (conv_hom ((Pi1^~ B)^~ s)) r1=>x y. exact: logical_step_pi1L.
+  apply: (conv_hom ((Pi1 A')^~ s)) r2=>x y. exact: logical_step_pi1R.
 Qed.
 
-Lemma sta_conv_sig0 A A' B B' s :
+Lemma logical_conv_sig0 A A' B B' s :
   A === A' -> B === B' -> Sig0 A B s === Sig0 A' B' s.
 Proof.
   move=> r1 r2.
   apply: (conv_trans (Sig0 A' B s)).
-  apply: (conv_hom ((Sig0^~ B)^~ s)) r1=>x y. exact: sta_step_sig0L.
-  apply: (conv_hom ((Sig0 A')^~ s)) r2=>x y. exact: sta_step_sig0R.
+  apply: (conv_hom ((Sig0^~ B)^~ s)) r1=>x y. exact: logical_step_sig0L.
+  apply: (conv_hom ((Sig0 A')^~ s)) r2=>x y. exact: logical_step_sig0R.
 Qed.
 
-Lemma sta_conv_sig1 A A' B B' s :
+Lemma logical_conv_sig1 A A' B B' s :
   A === A' -> B === B' -> Sig1 A B s === Sig1 A' B' s.
 Proof.
   move=> r1 r2.
   apply: (conv_trans (Sig1 A' B s)).
-  apply: (conv_hom ((Sig1^~ B)^~ s)) r1=>x y. exact: sta_step_sig1L.
-  apply: (conv_hom ((Sig1 A')^~ s)) r2=>x y. exact: sta_step_sig1R.
+  apply: (conv_hom ((Sig1^~ B)^~ s)) r1=>x y. exact: logical_step_sig1L.
+  apply: (conv_hom ((Sig1 A')^~ s)) r2=>x y. exact: logical_step_sig1R.
 Qed.
 
-Lemma sta_conv_pair0 m m' n n' t :
+Lemma logical_conv_pair0 m m' n n' t :
   m === m' -> n === n' -> Pair0 m n t === Pair0 m' n' t.
 Proof.
   move=>r1 r2.
   apply: (conv_trans (Pair0 m' n t)).
-  apply: (conv_hom ((Pair0^~ n)^~ t)) r1=>x y. exact: sta_step_pair0L.
-  apply: (conv_hom ((Pair0 m')^~ t)) r2=>x y. exact: sta_step_pair0R.
+  apply: (conv_hom ((Pair0^~ n)^~ t)) r1=>x y. exact: logical_step_pair0L.
+  apply: (conv_hom ((Pair0 m')^~ t)) r2=>x y. exact: logical_step_pair0R.
 Qed.
 
-Lemma sta_conv_pair1 m m' n n' t :
+Lemma logical_conv_pair1 m m' n n' t :
   m === m' -> n === n' -> Pair1 m n t === Pair1 m' n' t.
 Proof.
   move=>r1 r2.
   apply: (conv_trans (Pair1 m' n t)).
-  apply: (conv_hom ((Pair1^~ n)^~ t)) r1=>x y. exact: sta_step_pair1L.
-  apply: (conv_hom ((Pair1 m')^~ t)) r2=>x y. exact: sta_step_pair1R.
+  apply: (conv_hom ((Pair1^~ n)^~ t)) r1=>x y. exact: logical_step_pair1L.
+  apply: (conv_hom ((Pair1 m')^~ t)) r2=>x y. exact: logical_step_pair1R.
 Qed.
 
-Lemma sta_conv_letin A A' m m' n n' :
+Lemma logical_conv_letin A A' m m' n n' :
   A === A' -> m === m' -> n === n' -> LetIn A m n === LetIn A' m' n'.
 Proof.
   move=>r1 r2 r3.
   apply: (conv_trans (LetIn A' m n)).
-  apply: (conv_hom ((LetIn^~ m)^~ n)) r1=>x y. exact: sta_step_letinA.
+  apply: (conv_hom ((LetIn^~ m)^~ n)) r1=>x y. exact: logical_step_letinA.
   apply: (conv_trans (LetIn A' m' n)).
-  apply: (conv_hom (LetIn A'^~ n)) r2=>x y. exact: sta_step_letinL.
-  apply: (conv_hom (LetIn A' m')) r3=>x y. exact: sta_step_letinR.
+  apply: (conv_hom (LetIn A'^~ n)) r2=>x y. exact: logical_step_letinL.
+  apply: (conv_hom (LetIn A' m')) r3=>x y. exact: logical_step_letinR.
 Qed.
 
-Lemma sta_conv_with A A' B B' s :
+Lemma logical_conv_with A A' B B' s :
   A === A' -> B === B' -> With A B s === With A' B' s.
 Proof.
   move=>r1 r2.
   apply: (conv_trans (With A' B s)).
-  apply: (conv_hom ((With^~ B)^~ s)) r1=>x y. exact: sta_step_withL.
-  apply: (conv_hom ((With A')^~ s)) r2=>x y. exact: sta_step_withR.
+  apply: (conv_hom ((With^~ B)^~ s)) r1=>x y. exact: logical_step_withL.
+  apply: (conv_hom ((With A')^~ s)) r2=>x y. exact: logical_step_withR.
 Qed.
 
-Lemma sta_conv_apair m m' n n' s :
+Lemma logical_conv_apair m m' n n' s :
   m === m' -> n === n' -> APair m n s === APair m' n' s.
 Proof.
   move=>r1 r2.
   apply: (conv_trans (APair m' n s)).
-  apply: (conv_hom ((APair^~ n)^~ s)) r1=>x y. exact: sta_step_apairL.
-  apply: (conv_hom ((APair m')^~ s)) r2=>x y. exact: sta_step_apairR.
+  apply: (conv_hom ((APair^~ n)^~ s)) r1=>x y. exact: logical_step_apairL.
+  apply: (conv_hom ((APair m')^~ s)) r2=>x y. exact: logical_step_apairR.
 Qed.
 
-Lemma sta_conv_fst m m' :
+Lemma logical_conv_fst m m' :
   m === m' -> Fst m === Fst m'.
 Proof.
   move=>r.
-  apply: (conv_hom Fst) r=>x y. exact: sta_step_fst.
+  apply: (conv_hom Fst) r=>x y. exact: logical_step_fst.
 Qed.
 
-Lemma sta_conv_snd m m' :
+Lemma logical_conv_snd m m' :
   m === m' -> Snd m === Snd m'.
 Proof.
   move=>r.
-  apply: (conv_hom Snd) r=>x y. exact: sta_step_snd.
+  apply: (conv_hom Snd) r=>x y. exact: logical_step_snd.
 Qed.
 
-Lemma sta_conv_id A A' m m' n n' :
+Lemma logical_conv_id A A' m m' n n' :
   A === A' -> m === m' -> n === n' -> Id A m n === Id A' m' n'.
 Proof.
   move=>r1 r2 r3.
   apply: (conv_trans (Id A' m n)).
-  apply: (conv_hom ((Id^~ m)^~ n)) r1=>x y. exact: sta_step_idA.
+  apply: (conv_hom ((Id^~ m)^~ n)) r1=>x y. exact: logical_step_idA.
   apply: (conv_trans (Id A' m' n)).
-  apply: (conv_hom (Id A'^~ n)) r2=>x y. exact: sta_step_idL.
-  apply: (conv_hom (Id A' m')) r3=>x y. exact: sta_step_idR.
+  apply: (conv_hom (Id A'^~ n)) r2=>x y. exact: logical_step_idL.
+  apply: (conv_hom (Id A' m')) r3=>x y. exact: logical_step_idR.
 Qed.
 
-Lemma sta_conv_refl m m' :
+Lemma logical_conv_refl m m' :
   m === m' -> Refl m === Refl m'.
 Proof.
   move=>r.
-  apply: (conv_hom Refl) r=>x y. exact: sta_step_refl.
+  apply: (conv_hom Refl) r=>x y. exact: logical_step_refl.
 Qed.
 
-Lemma sta_conv_rw A A' H H' P P' :
+Lemma logical_conv_rw A A' H H' P P' :
   A === A' -> H === H' -> P === P' -> Rw A H P === Rw A' H' P'.
 Proof.
   move=>r1 r2 r3.
   apply: (conv_trans (Rw A' H P)).
-  apply: (conv_hom ((Rw^~ H)^~ P)) r1=>x y. exact: sta_step_rwA.
+  apply: (conv_hom ((Rw^~ H)^~ P)) r1=>x y. exact: logical_step_rwA.
   apply: (conv_trans (Rw A' H' P)).
-  apply: (conv_hom (Rw A'^~ P)) r2=>x y. exact: sta_step_rwH.
-  apply: (conv_hom (Rw A' H')) r3=>x y. exact: sta_step_rwP.
+  apply: (conv_hom (Rw A'^~ P)) r2=>x y. exact: logical_step_rwH.
+  apply: (conv_hom (Rw A' H')) r3=>x y. exact: logical_step_rwP.
 Qed.
 
-Lemma sta_conv_subst σ m n :
+Lemma logical_conv_subst σ m n :
   m === n -> m.[σ] === n.[σ].
 Proof.
   move=>c.
   apply: conv_hom c.
-  exact: sta_step_subst.
+  exact: logical_step_subst.
 Qed.
 
 Lemma sconv_up σ τ : sconv σ τ -> sconv (up σ) (up τ).
-Proof. move=> A [|x] //=. asimpl. exact: sta_conv_subst. Qed.
+Proof. move=> A [|x] //=. asimpl. exact: logical_conv_subst. Qed.
 
 Lemma sconv_upn n σ τ : sconv σ τ -> sconv (upn n σ) (upn n τ).
 Proof.
@@ -492,50 +496,50 @@ Proof.
 Qed.
 
 #[export] Hint Resolve
-  sta_conv_app
-  sta_conv_lam0 sta_conv_lam1
-  sta_conv_pi0 sta_conv_pi1
-  sta_conv_sig0 sta_conv_sig1
-  sta_conv_pair0 sta_conv_pair1
-  sta_conv_letin
-  sta_conv_with sta_conv_apair
-  sta_conv_fst sta_conv_snd
-  sta_conv_id sta_conv_refl sta_conv_rw
-  sconv_up sconv_upn : sta_conv_congr.
+  logical_conv_app
+  logical_conv_lam0 logical_conv_lam1
+  logical_conv_pi0 logical_conv_pi1
+  logical_conv_sig0 logical_conv_sig1
+  logical_conv_pair0 logical_conv_pair1
+  logical_conv_letin
+  logical_conv_with logical_conv_apair
+  logical_conv_fst logical_conv_snd
+  logical_conv_id logical_conv_refl logical_conv_rw
+  sconv_up sconv_upn : logical_conv_congr.
 
-Lemma sta_conv_compat σ τ s :
+Lemma logical_conv_compat σ τ s :
   sconv σ τ -> s.[σ] === s.[τ].
-Proof. elim: s σ τ => *; asimpl; eauto 9 with sta_conv_congr. Qed.
+Proof. elim: s σ τ => *; asimpl; eauto 9 with logical_conv_congr. Qed.
 
-Lemma sta_conv_beta m n1 n2 : n1 === n2 -> m.[n1/] === m.[n2/].
-Proof. move=> c. by apply: sta_conv_compat => -[]. Qed.
+Lemma logical_conv_beta m n1 n2 : n1 === n2 -> m.[n1/] === m.[n2/].
+Proof. move=> c. by apply: logical_conv_compat => -[]. Qed.
 
 Lemma pstep_reflexive m : pstep m m.
 Proof. elim: m; eauto using pstep. Qed.
 #[global] Hint Resolve pstep_reflexive.
 
-Lemma sta_step_pstep m m' : sta_step m m' -> pstep m m'.
+Lemma logical_step_pstep m m' : logical_step m m' -> pstep m m'.
 Proof with eauto using pstep, pstep_reflexive. elim... Qed.
 
-Lemma pstep_sta_red m n : pstep m n -> m ~>* n.
+Lemma pstep_logical_red m n : pstep m n -> m ~>* n.
 Proof with eauto.
-  elim=>{m n}//=; eauto with sta_red_congr.
+  elim=>{m n}//=; eauto with logical_red_congr.
   { move=> A m m' n n' s p1 r1 p2 r2.
     apply: starES. by constructor.
-    apply: (star_trans (m'.[n/])). exact: sta_red_subst.
-    by apply: sta_red_compat=>-[|]. }
+    apply: (star_trans (m'.[n/])). exact: logical_red_subst.
+    by apply: logical_red_compat=>-[|]. }
   { move=> A m m' n n' s p1 r1 p2 r2.
     apply: starES. by constructor.
-    apply: (star_trans (m'.[n/])). exact: sta_red_subst.
-    by apply: sta_red_compat=>-[|]. }
+    apply: (star_trans (m'.[n/])). exact: logical_red_subst.
+    by apply: logical_red_compat=>-[|]. }
   { move=> A m1 m1' m2 m2' n n' s p1 r1 p2 r2 p r.
     apply: starES. by constructor.
-    apply: (star_trans (n'.[m2,m1/])). exact: sta_red_subst.
-    by apply: sta_red_compat=>-[|-[]]. }
+    apply: (star_trans (n'.[m2,m1/])). exact: logical_red_subst.
+    by apply: logical_red_compat=>-[|-[]]. }
   { move=> A m1 m1' m2 m2' n n' s p1 r1 p2 r2 p r.
     apply: starES. by constructor.
-    apply: (star_trans (n'.[m2,m1/])). exact: sta_red_subst.
-    by apply: sta_red_compat=>-[|-[]]. }
+    apply: (star_trans (n'.[m2,m1/])). exact: logical_red_subst.
+    by apply: logical_red_compat=>-[|-[]]. }
   { move=>m m' n s p r.
     apply: starES. by constructor. eauto. }
   { move=>m m' n s p r.
@@ -622,6 +626,7 @@ Proof with eauto using pstep_compat, psstep_reflexive, psstep_compat.
   move...
 Qed.
 
+(* Diamond property for parallel reduction. *)
 Lemma pstep_diamond m m1 m2 :
   pstep m m1 -> pstep m m2 -> exists2 m', pstep m1 m' & pstep m2 m'.
 Proof with eauto 6 using
@@ -780,52 +785,53 @@ Lemma strip m m1 m2 :
   pstep m m1 -> m ~>* m2 -> exists2 m', m1 ~>* m' & pstep m2 m'.
 Proof with eauto using pstep_refl, star.
   move=>p r. elim: r m1 p=>{m2}...
-  move=>m1 m2 r1 ih /sta_step_pstep p1 m' p2.
+  move=>m1 m2 r1 ih /logical_step_pstep p1 m' p2.
   move:(ih _ p2)=>[m3 r2 p3].
   move:(pstep_diamond p1 p3)=>[m4 p4 p5].
   exists m4...
   apply: star_trans.
   apply: r2.
-  by apply: pstep_sta_red.
+  by apply: pstep_logical_red.
 Qed.
 
+(* Theorem 1 (Confluence of Logical Reductions) *)
 Theorem confluence :
-  confluent sta_step.
-Proof with eauto using sta_step, star.
+  confluent logical_step.
+Proof with eauto using logical_step, star.
   unfold confluent.
   unfold joinable.
   move=> x y z r.
   elim: r z=>{y}.
   move=>z r. exists z...
-  move=>y z r1 ih /sta_step_pstep p z0 /ih[z1 r2 r3].
+  move=>y z r1 ih /logical_step_pstep p z0 /ih[z1 r2 r3].
   move:(strip p r2)=>[z2 r4 p1].
   exists z2...
   apply: star_trans.
   apply r3.
-  apply: pstep_sta_red...
+  apply: pstep_logical_red...
 Qed.
 
 Theorem church_rosser :
-  CR sta_step.
+  CR logical_step.
 Proof.
   apply confluent_cr.
   apply confluence.
 Qed.
 
-Lemma sta_red_var_inv x y : Var x ~>* y -> y = Var x.
+Lemma logical_red_var_inv x y : Var x ~>* y -> y = Var x.
 Proof.
   elim=>//{} y z r1 e r2; subst.
   inv r2.
 Qed.
 
-Lemma sta_red_sort_inv s A :
+Lemma logical_red_sort_inv s A :
   Sort s ~>* A -> A = Sort s.
 Proof.
   elim=>//y z r1 e r2; subst.
   inv r2.
 Qed.
 
-Lemma sta_red_pi0_inv A B s x :
+Lemma logical_red_pi0_inv A B s x :
   Pi0 A B s ~>* x ->
   exists A' B',
     A ~>* A' /\ B ~>* B' /\ x = Pi0 A' B' s.
@@ -842,7 +848,7 @@ Proof.
   apply: starSE; eauto.
 Qed.
 
-Lemma sta_red_pi1_inv A B s x :
+Lemma logical_red_pi1_inv A B s x :
   Pi1 A B s ~>* x ->
   exists A' B',
     A ~>* A' /\ B ~>* B' /\ x = Pi1 A' B' s.
@@ -859,7 +865,7 @@ Proof.
   apply: starSE; eauto.
 Qed.
 
-Lemma sta_red_lam0_inv A m x s :
+Lemma logical_red_lam0_inv A m x s :
   Lam0 A m s ~>* x ->
   exists A' m',
     A ~>* A' /\ m ~>* m' /\ x = Lam0 A' m' s.
@@ -872,7 +878,7 @@ Proof.
   exists A'. exists m'0. eauto using star.
 Qed.
 
-Lemma sta_red_lam1_inv A m x s :
+Lemma logical_red_lam1_inv A m x s :
   Lam1 A m s ~>* x ->
   exists A' m',
     A ~>* A' /\ m ~>* m' /\ x = Lam1 A' m' s.
@@ -885,7 +891,7 @@ Proof.
   exists A'. exists m'0. eauto using star.
 Qed.
 
-Lemma sta_red_sig0_inv A B s x :
+Lemma logical_red_sig0_inv A B s x :
   Sig0 A B s ~>* x ->
   exists A' B',
     A ~>* A' /\ B ~>* B' /\ x = Sig0 A' B' s.
@@ -902,7 +908,7 @@ Proof.
   apply: starSE; eauto.
 Qed.
 
-Lemma sta_red_sig1_inv A B s x :
+Lemma logical_red_sig1_inv A B s x :
   Sig1 A B s ~>* x ->
   exists A' B',
     A ~>* A' /\ B ~>* B' /\ x = Sig1 A' B' s.
@@ -919,7 +925,7 @@ Proof.
   apply: starSE; eauto.
 Qed.
 
-Lemma sta_red_pair0_inv m n s x :
+Lemma logical_red_pair0_inv m n s x :
   Pair0 m n s ~>* x ->
   exists m' n',
     m ~>* m' /\ n ~>* n' /\ x = Pair0 m' n' s.
@@ -936,7 +942,7 @@ Proof.
   apply: starSE; eauto.
 Qed.
 
-Lemma sta_red_pair1_inv m n s x :
+Lemma logical_red_pair1_inv m n s x :
   Pair1 m n s ~>* x ->
   exists m' n',
     m ~>* m' /\ n ~>* n' /\ x = Pair1 m' n' s.
@@ -953,7 +959,7 @@ Proof.
   apply: starSE; eauto.
 Qed.
 
-Lemma sta_red_with_inv A B s x :
+Lemma logical_red_with_inv A B s x :
   With A B s ~>* x ->
   exists A' B',
     A ~>* A' /\ B ~>* B' /\ x = With A' B' s.
@@ -970,7 +976,7 @@ Proof.
   apply: starSE; eauto.
 Qed.
 
-Lemma sta_red_apair_inv m n s x :
+Lemma logical_red_apair_inv m n s x :
   APair m n s ~>* x ->
   exists m' n',
     m ~>* m' /\ n ~>* n' /\ x = APair m' n' s.
@@ -987,7 +993,7 @@ Proof.
   apply: starSE; eauto.
 Qed.
 
-Lemma sta_red_id_inv A m n x :
+Lemma logical_red_id_inv A m n x :
   Id A m n ~>* x ->
   exists A' m' n',
     A ~>* A' /\ m ~>* m' /\ n ~>* n' /\ x = Id A' m' n'.
@@ -1007,7 +1013,7 @@ Proof.
   apply: starSE; eauto.
 Qed.
 
-Lemma sta_red_refl_inv m x :
+Lemma logical_red_refl_inv m x :
   Refl m ~>* x ->
   exists m', m ~>* m' /\ x = Refl m'.
 Proof.
@@ -1022,7 +1028,7 @@ Qed.
 Lemma sort_inj s1 s2 :
   Sort s1 === Sort s2 -> s1 = s2.
 Proof.
-  move/church_rosser=>[x/sta_red_sort_inv->/sta_red_sort_inv[->]]//.
+  move/church_rosser=>[x/logical_red_sort_inv->/logical_red_sort_inv[->]]//.
 Qed.
 
 Lemma pi0_inj A A' B B' s s' :
@@ -1030,8 +1036,8 @@ Lemma pi0_inj A A' B B' s s' :
     A === A' /\ B === B' /\ s = s'.
 Proof.
   move/church_rosser=>
-    [x/sta_red_pi0_inv[A1[B1[rA1[rB1->]]]]
-      /sta_red_pi0_inv[A2[B2[rA2[rB2[]]]]]] eA eB es; subst.
+    [x/logical_red_pi0_inv[A1[B1[rA1[rB1->]]]]
+      /logical_red_pi0_inv[A2[B2[rA2[rB2[]]]]]] eA eB es; subst.
   repeat split.
   apply: conv_trans.
   apply: star_conv. by apply: rA1.
@@ -1046,8 +1052,8 @@ Lemma pi1_inj A A' B B' s s' :
     A === A' /\ B === B' /\ s = s'.
 Proof.
   move/church_rosser=>
-    [x/sta_red_pi1_inv[A1[B1[rA1[rB1->]]]]
-      /sta_red_pi1_inv[A2[B2[rA2[rB2[]]]]]] eA eB es; subst.
+    [x/logical_red_pi1_inv[A1[B1[rA1[rB1->]]]]
+      /logical_red_pi1_inv[A2[B2[rA2[rB2[]]]]]] eA eB es; subst.
   repeat split.
   apply: conv_trans.
   apply: star_conv. by apply: rA1.
@@ -1062,8 +1068,8 @@ Lemma sig0_inj A A' B B' s s' :
     A === A' /\ B === B' /\ s = s'.
 Proof.
   move/church_rosser=>
-    [x/sta_red_sig0_inv[A1[B1[rA1[rB1->]]]]
-      /sta_red_sig0_inv[A2[B2[rA2[rB2[]]]]]] eA eB es; subst.
+    [x/logical_red_sig0_inv[A1[B1[rA1[rB1->]]]]
+      /logical_red_sig0_inv[A2[B2[rA2[rB2[]]]]]] eA eB es; subst.
   repeat split.
   apply: conv_trans.
   apply: star_conv. by apply: rA1.
@@ -1078,8 +1084,8 @@ Lemma sig1_inj A A' B B' s s' :
     A === A' /\ B === B' /\ s = s'.
 Proof.
   move/church_rosser=>
-    [x/sta_red_sig1_inv[A1[B1[rA1[rB1->]]]]
-      /sta_red_sig1_inv[A2[B2[rA2[rB2[]]]]]] eA eB es; subst.
+    [x/logical_red_sig1_inv[A1[B1[rA1[rB1->]]]]
+      /logical_red_sig1_inv[A2[B2[rA2[rB2[]]]]]] eA eB es; subst.
   repeat split.
   apply: conv_trans.
   apply: star_conv. by apply: rA1.
@@ -1094,8 +1100,8 @@ Lemma with_inj A A' B B' s s' :
     A === A' /\ B === B' /\ s = s'.
 Proof.
   move/church_rosser=>
-    [x/sta_red_with_inv[A1[B1[rA1[rB1->]]]]
-      /sta_red_with_inv[A2[B2[rA2[rB2[]]]]]] eA eB es; subst.
+    [x/logical_red_with_inv[A1[B1[rA1[rB1->]]]]
+      /logical_red_with_inv[A2[B2[rA2[rB2[]]]]]] eA eB es; subst.
   repeat split.
   apply: conv_trans.
   apply: star_conv. by apply: rA1.
@@ -1110,8 +1116,8 @@ Lemma id_inj A A' m m' n n' :
     A === A' /\ m === m' /\ n === n'.
 Proof.
   move/church_rosser=>
-    [x/sta_red_id_inv[A1[m1[n1[rA1[rm1[rn1->]]]]]]
-      /sta_red_id_inv[A2[m2[n2[rA2[rm2[rn2[]]]]]]]] eA em en; subst.
+    [x/logical_red_id_inv[A1[m1[n1[rA1[rm1[rn1->]]]]]]
+      /logical_red_id_inv[A2[m2[n2[rA2[rm2[rn2[]]]]]]]] eA em en; subst.
   repeat split.
   apply: conv_trans.
   apply: star_conv. by apply: rA1.
@@ -1124,22 +1130,23 @@ Proof.
   apply: conv_sym. by apply: star_conv.
 Qed.
 
+(* Helpful tatics for the refutation of obvious inequalities. *)
 Ltac red_inv m H :=
   match m with
-  | Var   => apply sta_red_var_inv in H
-  | Sort  => apply sta_red_sort_inv in H
-  | Pi0   => apply sta_red_pi0_inv in H
-  | Pi1   => apply sta_red_pi1_inv in H
-  | Lam0  => apply sta_red_lam0_inv in H
-  | Lam1  => apply sta_red_lam1_inv in H
-  | Sig0  => apply sta_red_sig0_inv in H
-  | Sig1  => apply sta_red_sig1_inv in H
-  | Pair0 => apply sta_red_pair0_inv in H
-  | Pair1 => apply sta_red_pair1_inv in H
-  | With  => apply sta_red_with_inv in H
-  | APair => apply sta_red_apair_inv in H
-  | Id    => apply sta_red_id_inv in H
-  | Refl  => apply sta_red_refl_inv in H
+  | Var   => apply logical_red_var_inv in H
+  | Sort  => apply logical_red_sort_inv in H
+  | Pi0   => apply logical_red_pi0_inv in H
+  | Pi1   => apply logical_red_pi1_inv in H
+  | Lam0  => apply logical_red_lam0_inv in H
+  | Lam1  => apply logical_red_lam1_inv in H
+  | Sig0  => apply logical_red_sig0_inv in H
+  | Sig1  => apply logical_red_sig1_inv in H
+  | Pair0 => apply logical_red_pair0_inv in H
+  | Pair1 => apply logical_red_pair1_inv in H
+  | With  => apply logical_red_with_inv in H
+  | APair => apply logical_red_apair_inv in H
+  | Id    => apply logical_red_id_inv in H
+  | Refl  => apply logical_red_refl_inv in H
   end.
 
 Ltac solve_conv' :=
@@ -1149,12 +1156,12 @@ Ltac solve_conv' :=
     apply church_rosser in H; inv H
   end;
   repeat match goal with
-  | [ H : sta_red (?m _) _ |- _ ]         => red_inv m H
-  | [ H : sta_red (?m _ _) _ |- _ ]       => red_inv m H
-  | [ H : sta_red (?m _ _ _) _ |- _ ]     => red_inv m H
-  | [ H : sta_red (?m _ _ _ _) _ |- _ ]   => red_inv m H
-  | [ H : sta_red (?m _ _ _ _ _) _ |- _ ] => red_inv m H
-  | [ H : sta_red ?m _ |- _ ]             => red_inv m H
+  | [ H : logical_red (?m _) _ |- _ ]         => red_inv m H
+  | [ H : logical_red (?m _ _) _ |- _ ]       => red_inv m H
+  | [ H : logical_red (?m _ _ _) _ |- _ ]     => red_inv m H
+  | [ H : logical_red (?m _ _ _ _) _ |- _ ]   => red_inv m H
+  | [ H : logical_red (?m _ _ _ _ _) _ |- _ ] => red_inv m H
+  | [ H : logical_red ?m _ |- _ ]             => red_inv m H
   end;
   firstorder; subst;
   match goal with
