coq/theories/mltt_ast.v
@@ -1,3 +1,5 @@
+(* This file defines the abstract syntax of MLTT. *)
+
 From mathcomp Require Import ssreflect ssrbool eqtype ssrnat seq.
 From Coq Require Import ssrfun Classical Utf8.
 Require Export AutosubstSsr ARS.
@@ -6,6 +8,8 @@ Set Implicit Arguments.
 Unset Strict Implicit.
 Unset Printing Implicit Defensive.
 
+(* Abstract syntax tree of MLTT.
+   Variables are represented using DeBrujin indices. *)
 Inductive term : Type :=
 | Var (x : var)
 | Ty
@@ -15,14 +19,15 @@ Inductive term : Type :=
 | Sig (A : term) (B : {bind term}) (* Σ (x : A).B *)
 | DPair (m n : term) (* (m, n) *)
 | LetIn (A : {bind term}) (m : term) (n : {bind 2 of term}) (* RΣ([z]A, m, [x,y]n) *)
-| Tuple (A B : term) (* A×B *)
+| Tuple (A B : term) (* A × B *)
 | Pair (m n : term) (* (m, n) *)
 | Fst (m : term) (* π1 m *)
 | Snd (m : term) (* π2 m *)
-| Id (A m n : term)
+| Id (A m n : term) (* m =A n *)
 | Refl (m : term)
 | Rw (A : {bind 2 of term}) (H P : term) (* R=([x,p]A,H,P) *).
 
+(* Derive basic syntactic lemmas using autosubst. *)
 #[global] Instance Ids_term : Ids term. derive. Defined.
 #[global] Instance Rename_term : Rename term. derive. Defined.
 #[global] Instance Subst_term : Subst term. derive. Defined.
